theories/jessie/escrow2013_target.v
@@ -1,0 +1,173 @@
+From Coq Require Import List String ZArith.
+From iris.jessie Require Import jessica_ast.
+
+Import ListNotations.
+Open Scope string_scope.
+Open Scope Z_scope.
+
+Module Escrow2013Target.
+  Import JessicaAst.
+
+  Definition u (x : string) : jexpr := JUse x.
+  Definition s (x : string) : jexpr := JDataString x.
+  Definition n (x : Z) : jexpr := JDataNum x.
+  Definition arr (xs : list jexpr) : jexpr := JArray xs.
+  Definition def (x : string) : jpat := JDef x.
+  Definition bind (x : string) (rhs : jexpr) : jbind := JBind (def x) rhs.
+  Definition bind_pat (p : jpat) (rhs : jexpr) : jbind := JBind p rhs.
+  Definition prop (name : string) (value : jexpr) : jprop := JProp name value.
+  Definition get (obj : jexpr) (field : string) : jexpr := JGet obj field.
+  Definition call (callee : jexpr) (args : list jexpr) : jexpr := JCall callee args.
+  Definition callm (obj : jexpr) (field : string) (args : list jexpr) : jexpr :=
+    JCall (JGet obj field) args.
+  Definition arrow (params : list jpat) (ss : list jstmt) : jexpr :=
+    JArrow params (JBodyBlock ss).
+  Definition arrow_expr (params : list jpat) (e : jexpr) : jexpr :=
+    JArrow params (JBodyExpr e).
+  Definition lambda (params : list jpat) (ss : list jstmt) : jexpr :=
+    JLambda params (JBodyBlock ss).
+  Definition not_ (e : jexpr) : jexpr := JPreOp "!" e.
+
+  Definition qjoin_body : list jstmt :=
+    [ JReturn
+        (callm
+          (callm (u "Q") "all" [arr [u "p1"; u "p2"]])
+          "then"
+          [ arrow
+              [JMatchArray [def "r1"; def "r2"]]
+              [ JIf
+                  (not_ (callm (u "Object") "is" [u "r1"; u "r2"]))
+                  [JThrow (call (u "Error") [s "join failed"])]
+                  None;
+                JReturn (u "r1")
+              ]
+          ])
+    ].
+
+  Definition transfer_body : list jstmt :=
+    [ JConstStmt
+        [ bind
+            "makeEscrowPurseP"
+            (call (u "Qjoin")
+              [ get (callm (u "E") "get" [u "srcPurseP"]) "makePurse";
+                get (callm (u "E") "get" [u "dstPurseP"]) "makePurse"
+              ])
+        ];
+      JConstStmt
+        [ bind
+            "escrowPurseP"
+            (call (call (u "E") [u "makeEscrowPurseP"]) [])
+        ];
+      JExprStmt
+        (callm
+          (call (u "Q") [u "decisionP"])
+          "then"
+          [ arrow [def "_"]
+              [ JExprStmt
+                  (callm
+                    (call (u "E") [u "dstPurseP"])
+                    "deposit"
+                    [u "amount"; u "escrowPurseP"])
+              ];
+            arrow [def "_"]
+              [ JExprStmt
+                  (callm
+                    (call (u "E") [u "srcPurseP"])
+                    "deposit"
+                    [u "amount"; u "escrowPurseP"])
+              ]
+          ]);
+      JReturn
+        (callm
+          (call (u "E") [u "escrowPurseP"])
+          "deposit"
+          [u "amount"; u "srcPurseP"])
+    ].
+
+  Definition failOnly_body : list jstmt :=
+    [ JReturn
+        (callm
+          (call (u "Q") [u "cancellationP"])
+          "then"
+          [ arrow [def "cancellation"]
+              [JThrow (u "cancellation")]
+          ])
+    ].
+
+  Definition escrowExchange_body : list jstmt :=
+    [ JLetNames [def "decide"];
+      JConstStmt
+        [ bind
+            "decisionP"
+            (callm
+              (u "Q")
+              "promise"
+              [ arrow [def "resolve"]
+                  [JExprStmt (JAssign (u "decide") (u "resolve"))]
+              ])
+        ];
+      JExprStmt
+        (call
+          (u "decide")
+          [ callm
+              (u "Q")
+              "race"
+              [ arr
+                  [ callm
+                      (u "Q")
+                      "all"
+                      [ arr
+                          [ call (u "transfer")
+                              [ u "decisionP";
+                                get (u "a") "moneySrcP";
+                                get (u "b") "moneyDstP";
+                                get (u "b") "moneyNeeded"
+                              ];
+                            call (u "transfer")
+                              [ u "decisionP";
+                                get (u "b") "stockSrcP";
+                                get (u "a") "stockDstP";
+                                get (u "a") "stockNeeded"
+                              ]
+                          ]
+                      ];
+                    call (u "failOnly") [get (u "a") "cancellationP"];
+                    call (u "failOnly") [get (u "b") "cancellationP"]
+                  ]
+              ]
+          ]);
+      JReturn (u "decisionP")
+    ].
+
+  Definition escrow2013_program : jmodule :=
+    JModule
+      [ JImport [JImportAs "E" "E"] "@endo/far";
+        JConst [bind "Q" (u "Promise")];
+        JConst
+          [ bind
+              "Qjoin"
+              (call (u "harden")
+                [ JLambda [def "p1"; def "p2"] (JBodyBlock qjoin_body) ])
+          ];
+        JConst
+          [ bind
+              "transfer"
+              (call (u "harden")
+                [ JArrow
+                    [def "decisionP"; def "srcPurseP"; def "dstPurseP"; def "amount"]
+                    (JBodyBlock transfer_body) ])
+          ];
+        JConst
+          [ bind
+              "failOnly"
+              (call (u "harden")
+                [ JLambda [def "cancellationP"] (JBodyBlock failOnly_body) ])
+          ];
+        JConst
+          [ bind
+              "escrowExchange"
+              (call (u "harden")
+                [ JArrow [def "a"; def "b"] (JBodyBlock escrowExchange_body) ])
+          ]
+      ].
+End Escrow2013Target.
