theories/jessie/peg/suffix.v
@@ -1,0 +1,132 @@
+From Coq Require Import Strings.String.
+
+Inductive suffix : string -> string -> Prop :=
+  | SuffixRefl :
+      forall s,
+      suffix s s
+  | SuffixChar :
+      forall s1 s2 a,
+      suffix s1 s2 ->
+      suffix s1 (String a s2).
+
+Lemma suffix_correct :
+  forall s1 s2,
+  suffix s1 (append s2 s1).
+Proof.
+  intros.
+  induction s2.
+  - constructor.
+  - simpl.
+    constructor.
+    trivial.
+Qed.
+
+Lemma suffix_trans :
+  forall s1 s2 s3,
+  suffix s1 s2 ->
+  suffix s2 s3 ->
+  suffix s1 s3.
+Proof.
+  intros.
+  generalize dependent s2.
+  generalize dependent s1.
+  induction s3 as [|a s3 IH]; intros s1 s2 H12 H23;
+  inversion H23; subst; auto.
+  constructor.
+  eauto using IH.
+Qed.
+
+Lemma suffix_length_le :
+  forall s1 s2,
+  suffix s1 s2 ->
+  length s1 <= length s2.
+Proof.
+  intros * H.
+  induction H; simpl; auto.
+Qed.
+
+Lemma suffix_length_eq :
+  forall s1 s2,
+  suffix s1 s2 ->
+  length s1 = length s2 ->
+  s1 = s2.
+Proof.
+  intros * H1 H2.
+  induction H1; auto.
+  specialize (suffix_length_le _ _ H1) as Hle.
+  rewrite H2 in Hle.
+  simpl in Hle.
+  exfalso.
+  apply (PeanoNat.Nat.nle_succ_diag_l _ Hle).
+Qed.
+
+Lemma suffix_antisymmetric :
+  forall s1 s2,
+  suffix s1 s2 ->
+  suffix s2 s1 ->
+  s1 = s2.
+Proof.
+  intros * H12 H21.
+  specialize (suffix_length_le _ _ H12) as Hlen12.
+  specialize (suffix_length_le _ _ H21) as Hlen21.
+  specialize (PeanoNat.Nat.le_antisymm _ _ Hlen12 Hlen21) as Hlen.
+  eauto using suffix_length_eq.
+Qed.
+
+Inductive proper_suffix : string -> string -> Prop :=
+  | ProperSuffixBase :
+      forall s a,
+      proper_suffix s (String a s)
+  | ProperSuffixRec :
+      forall s1 s2 a,
+      proper_suffix s1 s2 ->
+      proper_suffix s1 (String a s2)
+  .
+
+Lemma proper_suffix_length_lt :
+  forall s1 s2,
+  proper_suffix s1 s2 ->
+  length s1 < length s2.
+Proof.
+  intros * H.
+  induction H; simpl; auto.
+Qed.
+
+Lemma suffix_is_proper_suffix_with_char :
+  forall s1 s2 a,
+  suffix s1 s2 ->
+  proper_suffix s1 (String a s2).
+Proof.
+  intros * H.
+  generalize dependent a.
+  induction H;
+  eauto using proper_suffix.
+Qed.
+
+Lemma suffix_is_refl_or_proper_suffix :
+  forall s1 s2,
+  suffix s1 s2 ->
+  s1 = s2 \/ proper_suffix s1 s2.
+Proof.
+  intros * H.
+  inversion H; subst;
+  eauto using suffix_is_proper_suffix_with_char.
+Qed.
+
+Lemma proper_suffix_exists_append :
+  forall s1 s2,
+  proper_suffix s1 s2 ->
+  exists a s0, String a (s0 ++ s1) = s2.
+Proof.
+  intros * H.
+  induction H as [? a|? ? a ? [a' [s' ?]]].
+  - (* ProperSuffixBase *)
+    exists a.
+    exists EmptyString.
+    auto.
+  - (* ProperSuffixRec *)
+    subst.
+    exists a.
+    exists (String a' s').
+    auto.
+Qed.
