theories/jessie/peg/syntax.v
@@ -1,0 +1,99 @@
+From Coq Require Import Strings.Ascii.
+From Coq Require Import Lists.List.
+From Coq Require Import Lia.
+From iris.jessie.peg Require Import charset.
+
+(** Pattern (a.k.a. expression) **)
+
+Inductive pat : Type :=
+  | PEmpty : pat                          (* ε            *)
+  | PSet : charset -> pat                 (* [set]        *)
+  | PSequence : pat -> pat -> pat         (* p1 p2        *)
+  | PChoice : pat -> pat -> pat           (* p1 / p2      *)
+  | PRepetition : pat -> pat              (* p*           *)
+  | PNot : pat -> pat                     (* !p           *)
+  | PAnd : pat -> pat                     (* &p           *)
+  | PNT : nat -> pat                      (* G[i]         *)
+  .
+
+Fixpoint pat_size p :=
+  match p with
+  | PEmpty => 1
+  | PSet _ => 1
+  | PSequence p1 p2 => 1 + pat_size p1 + pat_size p2
+  | PChoice p1 p2 => 1 + pat_size p1 + pat_size p2
+  | PRepetition p => 1 + pat_size p
+  | PNot p => 1 + pat_size p
+  | PAnd p => 1 + pat_size p
+  | PNT _ => 1
+  end.
+
+Definition tocharset p : option charset :=
+  match p with
+  | PSet cs => Some cs
+  | _ => None
+  end.
+
+Inductive pat_le (p : pat) : pat -> Prop :=
+  | PLERefl :
+      pat_le p p
+  | PLESequence1 :
+      forall p1 p2,
+      pat_le p p1 ->
+      pat_le p (PSequence p1 p2)
+  | PLESequence2 :
+      forall p1 p2,
+      pat_le p p2 ->
+      pat_le p (PSequence p1 p2)
+  | PLEChoice1 :
+      forall p1 p2,
+      pat_le p p1 ->
+      pat_le p (PChoice p1 p2)
+  | PLEChoice2 :
+      forall p1 p2,
+      pat_le p p2 ->
+      pat_le p (PChoice p1 p2)
+  | PLERepetition :
+      forall p1,
+      pat_le p p1 ->
+      pat_le p (PRepetition p1)
+  | PLENot :
+      forall p1,
+      pat_le p p1 ->
+      pat_le p (PNot p1)
+  | PLEAnd :
+      forall p1,
+      pat_le p p1 ->
+      pat_le p (PAnd p1)
+  .
+
+(** Grammar **)
+
+Definition grammar : Type := list pat.
+
+Fixpoint grammar_size g :=
+  match g with
+  | cons p g' => pat_size p + grammar_size g'
+  | nil => 0
+  end.
+
+Lemma pat_size_le_grammar_size :
+  forall p g,
+  In p g ->
+  pat_size p <= grammar_size g.
+Proof.
+  intros * HIn.
+  generalize dependent p.
+  induction g as [|p' g' IHg]; intros.
+  + (* nil *)
+    inversion HIn.
+  + (* cons p' g' *)
+    inversion HIn as [|HIn']; subst.
+    - (* p = p' *)
+      simpl.
+      lia.
+    - (* In p (p' :: g') *)
+      simpl.
+      specialize (IHg _ HIn').
+      lia.
+Qed.
